Ongoing brainstorm for the proof of combinators

examples/Imp2Vir/Semantics.v
@@ -14,7 +14,7 @@ From Vellvm Require Import
      Semantics
      Syntax
      Syntax.ScopeTheory.
-From tutorial Require Import Fin Imp.
+From Imp2Vir Require Import Fin Imp.
 
 Require Import Vec Unique CvirCombinators CvirCombinatorsWF CompileExpr Imp2Cvir.
 
@@ -33,12 +33,64 @@ Definition R
   Prop :=
   Rmem (fst env1) vmap (fst (snd env2)) (fst env2).
 
+(* Denotation of a [cvir] construct.
+  Note: we should be able to take any three disjoint sets 
+  of names [vi,vo,vt] to feed our [ir].
+  One way is to take as a "canonical" name the first integers:
+  this is what the current version does with [build_map].
+  Another would be to be parameterized by three such sets ---
+  lemmas about it would assume that they are disjoint.
+  We currently suspect that the later formulation might be
+  necessary to express generic lemmas, even if "at the top level"
+  we will always use the canonical naming. It is not yet clear though. 
+*)
+Definition build_map a b :=
+  map Anon (map Z.of_nat (seq a b)).
+
 Definition denote_cvir {ni no} (ir : cvir ni no) (bid : fin ni) bid' :=
-  let vi := map Anon (map Z.of_nat (seq 0 ni)) in
-  let vo := map Anon (map Z.of_nat (seq ni no)) in
-  let vt := map Anon (map Z.of_nat (seq (ni + no) (n_int ir))) in
+  let vi := build_map 0 ni in
+  let vo := build_map ni no in
+  let vt := build_map (ni + no) (n_int ir) in
   denote_ocfg (convert_typ nil (blocks ir vi vo vt)) (bid', nth vi bid).
 
+(* In particular: can we have a reasoning principle to prove that two
+  cvir are related?
+  That is a lemma that would allow us to conclude something along the lines of:
+  [eutt R (denote_cvir ir1 n org) (denote_cvir ir2 m org)]
+  by chosing an invariant I and having two proof obligations:
+  - I holds initially (of n m and org?)
+  - If we start from arguments in I, then we prove something about
+  ir1.(blocks) and ir2.(blocks) at these arguments.
+
+This lemma would likely be based on and ressemble the low level lemma on [iter],
+but could be more precise since we are here considering bodies of a specific shape:
+
+Lemma eutt_iter_gen :
+forall {F : Type -> Type} {A B : Type} {R : A -> A -> Prop} {S : B -> B -> Prop},
+  forall body1 body2,
+   (forall a a', R a a' -> eutt (sum_rel R S) (body1 a) (body2 a')) ->
+   forall  a a', R a a' -> eutt S (iter body1 a) (iter body2 a')
+
+The drafted proof below of [denote_cvir_merge] uses [eutt_iter_gen] but
+leads to some non-trivial arithmetic and reasoning on renaming.
+Maybe using this hypothetical higher level lemma could sooth the pain.
+ *)
+
+(* The following lemmas should be true *)
+Lemma firstn_build_map : forall i n m,
+firstn n (build_map i (n + m)) = build_map i n.
+Admitted.
+
+Lemma skipn_build_map : forall i n m,
+skipn n (build_map i (n + m)) = build_map (i + n) m.
+Admitted.
+
+From Coq Require Import Morphisms.
+Require Import ITree.Basics.HeterogeneousRelations.
+Import ITreeNotations.
+Import SemNotations.
+
+(*  *)
 Theorem denote_cvir_merge : forall ni1 no1 ni2 no2 (ir1 : cvir ni1 no1) (ir2 : cvir ni2 no2) bid bid',
   cvir_ids_WF ir1 ->
   cvir_ids_WF ir2 ->
@@ -51,11 +103,94 @@ Theorem denote_cvir_merge : forall ni1 no1 ni2 no2 (ir1 : cvir ni1 no1) (ir2 : c
     | inr bid2 => denote_cvir ir2 bid2 bid'
     end).
 Proof.
-  intros.
-  unfold denote_cvir.
+  intros * WF11 WF12 WF21 WF22.
+  (* case analysis on which subgraph we are in: *)
+  destruct (split_fin_sum ni1 ni2 bid) eqn:Eq. 
+  - rename f into bid1. 
+    unfold denote_cvir.
+    unfold merge_cvir.
+    cbn.
+    rewrite !firstn_build_map.
+    rewrite !skipn_build_map.
+    (* the invariant on the block identifiers we encounter during the computation *)
+    set (I := (fun (fto fto' : block_id * block_id) =>
+        ( exists k, snd fto' = Anon (Z.of_nat k) /\
+                    snd fto = Anon (Z.of_nat k)  /\
+                    k < ni1
+         ) \/
+        (exists k, snd fto' = Anon (Z.of_nat k) /\ 
+                   snd fto  = Anon (Z.of_nat (k + ni2 + no2)) /\ 
+                   k >= ni1 + no1 
+                   (* Need for upper bound: k < ni1 + no1 + nt1? *)
+    ))%nat).
+    (* we apply [eutt_iter_gen] with this invariant *)
+    apply (@KTreeFacts.eutt_iter_gen _ _ _ I). 
+    + (* We need to prove that it is indeed an invariant *)
+      simpl bind.
+      intros [? ?b1] [? ?b2] HI.
+      destruct HI as [HI | HI].
+      * destruct HI as (k & EQ1 & EQ2 & INEQ); cbn in * |-.
+        (* 
+  Step 1: renaming and lookups
+ 
+  find_block
+      (convert_typ nil
+         (blocks ir1 (build_map 0 ni1) (build_map (ni1 + ni2) no1)
+            (build_map (ni1 + ni2 + (no1 + no2)) (n_int ir1)) ++
+          blocks ir2 (build_map (0 + ni1) ni2)
+            (build_map (ni1 + ni2 + no1) no2)
+            (build_map (ni1 + ni2 + (no1 + no2) + n_int ir1) (n_int ir2)))%list)
+      b1 = Some bk_src1
+
+find_block
+      (convert_typ nil
+         (blocks ir1 (build_map 0 ni1) (build_map ni1 no1)
+            (build_map (ni1 + no1) (n_int ir1)))) b2 = Some bk_src2
+
+  bk_src2 = rename_bk (to_write ) bk_src1
+
+  Step 2 : correctness of renaming
+    eutt (sum_rel rename_bid eq) bk (rename_bk bk)
+ *)
+        admit.
+      * admit.
+    + (* The invariant holds initially *)
+      admit.
+- admit.
+Admitted.
+
+
+  (*
+  Approach started by Nicolas:
+
+  clear f to FIND; intros fto fto' [-> FIND]; destruct fto as [f to] .
+  cbn in *.
+  epose proof (find_block_none_app _ bks2 _ FIND) as FIND_L1L2.
+  rewrite FIND_L1L2.
+  destruct (find_block bks2 to) eqn:FIND_L2.
+  - eapply eutt_post_bind.
+    apply denote_bk_exits_in_outputs.
+    intros [id | v] ?; cbn; apply eutt_Ret; eauto.
+    eapply inl_morphism; split; auto.
+    eapply find_block_not_in_inputs,no_reentrance_not_in; eauto.
+    eapply In_bk_outputs; eauto.
+*)
+
+(* 
+I (_, x)
+  nth vnth vi bigi bid
+
+  I : (block_id * block_id) -> (block_id * block_id) -> Prop
+  I ids1 ids2 -> eutt I ([|G1[snd ids1]|] (fst ids1)) ([|G1[snd ids2]|] (fst ids2))
+  I idsinit2 idsinit2
+  ---------
+  G1 idsinit2 ~ G2 idsinit2
+
+
   simpl.
   destruct (split_fin_sum _ _ _).
 Admitted.
+*)
 
 Definition sym_fin {n1 n2 n3 : nat} (f : fin (n1 + (n2 + n3))) : fin (n1 + (n3 + n2)) :=
   match split_fin_sum _ _ f with
@@ -92,3 +227,4 @@ Theorem compile_seq_correct : forall next_reg l r env next_reg' env' ir mem bid 
   (interp_imp (denote_imp (Seq l r)) mem)
   (interp_cfg3 (denote_cvir ir f0 bid) genv lenv vmem).
 Admitted.
+
